backend/Linear_coop.v
@@ -75,65 +75,60 @@ Definition parent_locset0 (ls0: locset) (stack: list Linear.stackframe) : locset
   | Linear.Stackframe f sp ls c :: stack' => ls
   end.
 
-Section RELSEM.
+Section LINEAR_COOP.
+Variable hf : I64Helpers.helper_functions.
 
-Variable ge: genv.
-
-Inductive Linear_step: Linear_core -> mem -> Linear_core -> mem -> Prop :=
+Inductive Linear_step (ge:genv): Linear_core -> mem -> Linear_core -> mem -> Prop :=
   | lin_exec_Lgetstack:
       forall s f sp sl ofs ty dst b rs m rs' lf,
       rs' = Locmap.set (R dst) (rs (S sl ofs ty)) (undef_regs (destroyed_by_getstack sl) rs) ->
-      Linear_step (Linear_State s f sp (Lgetstack sl ofs ty dst :: b) rs lf) m
+      Linear_step ge (Linear_State s f sp (Lgetstack sl ofs ty dst :: b) rs lf) m
         (Linear_State s f sp b rs' lf) m
   | lin_exec_Lsetstack:
       forall s f sp src sl ofs ty b rs m rs' lf,
       rs' = Locmap.set (S sl ofs ty) (rs (R src)) (undef_regs (destroyed_by_setstack ty) rs) ->
-      Linear_step (Linear_State s f sp (Lsetstack src sl ofs ty :: b) rs lf) m
+      Linear_step ge (Linear_State s f sp (Lsetstack src sl ofs ty :: b) rs lf) m
         (Linear_State s f sp b rs' lf) m
   | lin_exec_Lop:
       forall s f sp op args res b rs m v rs' lf,
       eval_operation ge sp op (reglist rs args) m = Some v ->
       rs' = Locmap.set (R res) v (undef_regs (destroyed_by_op op) rs) ->
-      Linear_step (Linear_State s f sp (Lop op args res :: b) rs lf) m
+      Linear_step ge (Linear_State s f sp (Lop op args res :: b) rs lf) m
         (Linear_State s f sp b rs' lf) m
   | lin_exec_Lload:
       forall s f sp chunk addr args dst b rs m a v rs' lf,
       eval_addressing ge sp addr (reglist rs args) = Some a ->
       Mem.loadv chunk m a = Some v ->
       rs' = Locmap.set (R dst) v (undef_regs (destroyed_by_load chunk addr) rs) ->
-      Linear_step (Linear_State s f sp (Lload chunk addr args dst :: b) rs lf) m
+      Linear_step ge (Linear_State s f sp (Lload chunk addr args dst :: b) rs lf) m
         (Linear_State s f sp b rs' lf) m
   | lin_exec_Lstore:
       forall s f sp chunk addr args src b rs m m' a rs' lf,
       eval_addressing ge sp addr (reglist rs args) = Some a ->
       Mem.storev chunk m a (rs (R src)) = Some m' ->
       rs' = undef_regs (destroyed_by_store chunk addr) rs ->
-      Linear_step (Linear_State s f sp (Lstore chunk addr args src :: b) rs lf) m
+      Linear_step ge (Linear_State s f sp (Lstore chunk addr args src :: b) rs lf) m
         (Linear_State s f sp b rs' lf) m'
   | lin_exec_Lcall:
       forall s f sp sig ros b rs m f' lf,
       find_function ge ros rs = Some f' ->
       sig = funsig f' ->
-      Linear_step (Linear_State s f sp (Lcall sig ros :: b) rs lf) m
+      Linear_step ge (Linear_State s f sp (Lcall sig ros :: b) rs lf) m
         (Linear_Callstate (Stackframe f sp rs b:: s) f' rs lf) m
   | lin_exec_Ltailcall:
       forall s f stk sig ros b rs m rs' f' m' rs0 f0,
       rs' = return_regs (parent_locset0 rs0 s) rs ->
       find_function ge ros rs' = Some f' ->
-      (*Lenb: Mach's at/after external treatment, and absence of m and ge in atExternal
-           may need this:
-           only internal calls can be tailcalls 
-            (exists f'', f' = Internal f'') ->*)
       sig = funsig f' ->
       Mem.free m stk 0 f.(fn_stacksize) = Some m' ->
-      Linear_step (Linear_State s f (Vptr stk Int.zero) (Ltailcall sig ros :: b) rs (mk_load_frame rs0 f0)) m
+      Linear_step ge (Linear_State s f (Vptr stk Int.zero) (Ltailcall sig ros :: b) rs (mk_load_frame rs0 f0)) m
         (Linear_Callstate s f' rs' (mk_load_frame rs0 f0)) m'
   | lin_exec_Lbuiltin:
       forall s f sp rs m ef args res b t vl rs' m' lf,
       external_call' ef ge (reglist rs args) m t vl m' ->
-      observableEF ef = false ->
+      observableEF hf ef = false ->
       rs' = Locmap.setlist (map R res) vl (undef_regs (destroyed_by_builtin ef) rs) ->
-      Linear_step (Linear_State s f sp (Lbuiltin ef args res :: b) rs lf) m
+      Linear_step ge (Linear_State s f sp (Lbuiltin ef args res :: b) rs lf) m
          (Linear_State s f sp b rs' lf) m'
 (*NO ANNOTS YET
   | lin_exec_Lannot:
@@ -143,25 +138,25 @@ Inductive Linear_step: Linear_core -> mem -> Linear_core -> mem -> Prop :=
          (Linear_State s f sp b rs) m'*)
   | lin_exec_Llabel:
       forall s f sp lbl b rs m lf,
-      Linear_step (Linear_State s f sp (Llabel lbl :: b) rs lf) m
+      Linear_step ge (Linear_State s f sp (Llabel lbl :: b) rs lf) m
         (Linear_State s f sp b rs lf) m
   | lin_exec_Lgoto:
       forall s f sp lbl b rs m b' lf,
       find_label lbl f.(fn_code) = Some b' ->
-      Linear_step (Linear_State s f sp (Lgoto lbl :: b) rs lf) m
+      Linear_step ge (Linear_State s f sp (Lgoto lbl :: b) rs lf) m
         (Linear_State s f sp b' rs lf) m
   | lin_exec_Lcond_true:
       forall s f sp cond args lbl b rs m rs' b' lf,
       eval_condition cond (reglist rs args) m = Some true ->
       rs' = undef_regs (destroyed_by_cond cond) rs ->
       find_label lbl f.(fn_code) = Some b' ->
-      Linear_step (Linear_State s f sp (Lcond cond args lbl :: b) rs lf) m
+      Linear_step ge (Linear_State s f sp (Lcond cond args lbl :: b) rs lf) m
         (Linear_State s f sp b' rs' lf) m
   | lin_exec_Lcond_false:
       forall s f sp cond args lbl b rs m rs' lf,
       eval_condition cond (reglist rs args) m = Some false ->
       rs' = undef_regs (destroyed_by_cond cond) rs ->
-      Linear_step (Linear_State s f sp (Lcond cond args lbl :: b) rs lf) m
+      Linear_step ge (Linear_State s f sp (Lcond cond args lbl :: b) rs lf) m
         (Linear_State s f sp b rs' lf) m
   | lin_exec_Ljumptable:
       forall s f sp arg tbl b rs m n lbl b' rs' lf,
@@ -169,39 +164,39 @@ Inductive Linear_step: Linear_core -> mem -> Linear_core -> mem -> Prop :=
       list_nth_z tbl (Int.unsigned n) = Some lbl ->
       find_label lbl f.(fn_code) = Some b' ->
       rs' = undef_regs (destroyed_by_jumptable) rs ->
-      Linear_step (Linear_State s f sp (Ljumptable arg tbl :: b) rs lf) m
+      Linear_step ge (Linear_State s f sp (Ljumptable arg tbl :: b) rs lf) m
         (Linear_State s f sp b' rs' lf) m
   | lin_exec_Lreturn:
       forall s f stk b rs m m' rs0 f0,
       let lf := mk_load_frame rs0 f0 in 
       Mem.free m stk 0 f.(fn_stacksize) = Some m' ->
-      Linear_step (Linear_State s f (Vptr stk Int.zero) (Lreturn :: b) rs lf) m
+      Linear_step ge (Linear_State s f (Vptr stk Int.zero) (Lreturn :: b) rs lf) m
         (Linear_Returnstate s (sig_res (fn_sig f)) (return_regs (parent_locset0 rs0 s) rs) lf) m'
   (*A dummy corestep, to facilitate the stacking proof.*)
   | lin_exec_function_internal0:
       forall s f rs m rs0 f0,
-      Linear_step (Linear_CallstateIn s (Internal f) rs (mk_load_frame rs0 f0)) m
+      Linear_step ge (Linear_CallstateIn s (Internal f) rs (mk_load_frame rs0 f0)) m
                   (Linear_Callstate s (Internal f) rs (mk_load_frame (call_regs rs0) f0)) m
   | lin_exec_function_internal:
       forall s f rs m rs' m' stk lf,
       Mem.alloc m 0 f.(fn_stacksize) = (m', stk) ->
       rs' = undef_regs destroyed_at_function_entry (call_regs rs) ->
-      Linear_step (Linear_Callstate s (Internal f) rs lf) m
+      Linear_step ge (Linear_Callstate s (Internal f) rs lf) m
         (Linear_State s f (Vptr stk Int.zero) f.(fn_code) rs' lf) m'
-(*NO RULE FOR EXTERNAL CALLS
+
   | lin_exec_function_external:
-      forall s ef args res rs1 rs2 m t m',
+      forall s ef args res rs1 rs2 m t m' lf
+      (OBS: observableEF hf ef = false),
       args = map rs1 (loc_arguments (ef_sig ef)) ->
       external_call' ef ge args m t res m' ->
       rs2 = Locmap.setlist (map R (loc_result (ef_sig ef))) res rs1 ->
-      Linear_step (Linear_Callstate s (External ef) rs1) m
-          (Linear_Returnstate s rs2) m'*)
+      Linear_step ge (Linear_Callstate s (External ef) rs1 lf) m
+          (Linear_Returnstate s (sig_res (ef_sig ef)) rs2 lf) m'
+
   | lin_exec_return:
       forall s f sp lf c rs retty m rs_init,
-      Linear_step (Linear_Returnstate (Stackframe f sp lf c :: s) retty rs rs_init) m
+      Linear_step ge (Linear_Returnstate (Stackframe f sp lf c :: s) retty rs rs_init) m
          (Linear_State s f sp c rs rs_init) m.
-
-End RELSEM.
 
 Definition init_locset tys args :=
   Locmap.setlist (loc_arguments_rec tys 0) (encode_longs tys args) (Locmap.init Vundef).
@@ -283,7 +278,7 @@ Definition Linear_at_external (c: Linear_core) : option (external_function * sig
       match f with
         | Internal f => None
         | External ef => 
-            if observableEF ef
+            if observableEF hf ef
             then Some (ef, ef_sig ef, decode_longs (sig_args (ef_sig ef)) 
                                    (map rs (loc_arguments (ef_sig ef))))
             else None
@@ -310,19 +305,20 @@ Definition Linear_after_external (vret: option val) (c: Linear_core) : option Li
     | _ => None
   end.
 
-Lemma Linear_corestep_not_at_external:
-       forall ge m q m' q', Linear_step ge q m q' m' -> Linear_at_external q = None.
-  Proof. intros. inv H; try reflexivity. Qed.
+Lemma Linear_corestep_not_at_external ge m q m' q':
+      Linear_step ge q m q' m' -> Linear_at_external q = None.
+  Proof. intros. inv H; try reflexivity. 
+    simpl. rewrite OBS. trivial. Qed.
 
-Lemma Linear_corestep_not_halted : forall ge m q m' q', 
+Lemma Linear_corestep_not_halted ge m q m' q' :
        Linear_step ge q m q' m' -> Linear_halted q = None.
   Proof. intros. inv H; reflexivity. Qed.
     
-Lemma Linear_at_external_halted_excl :
-       forall q, Linear_at_external q = None \/ Linear_halted q = None.
+Lemma Linear_at_external_halted_excl q:
+      Linear_at_external q = None \/ Linear_halted q = None.
    Proof. intros. destruct q; auto. Qed.
 
-Lemma Linear_after_at_external_excl : forall retv q q',
+Lemma Linear_after_at_external_excl retv q q':
       Linear_after_external retv q = Some q' -> Linear_at_external q' = None.
   Proof. intros.
        destruct q; simpl in *; try inv H.
@@ -363,6 +359,8 @@ Lemma Linear_forward : forall g c m c' m' (CS: Linear_step g c m c' m'),
            eapply free_forward; eassumption.
          (*internal function*)
            eapply alloc_forward; eassumption.
+         (*external unobservable function*)
+           inv H0. eapply external_call_mem_forward; eassumption.
 Qed.
 
 Program Definition Linear_coop_sem : 
@@ -371,3 +369,4 @@ apply Build_CoopCoreSem with (coopsem := Linear_core_sem).
   apply Linear_forward.
 Defined.
 
+End LINEAR_COOP.
