backend/Linear_eff.v
@@ -9,6 +9,7 @@ Require Import Globalenvs.
 
 Require Import Op.
 Require Import Locations.
+Require Import Conventions.
 Require Import LTL. (*for undef_regs etc*)
 
 Require Import mem_lemmas. (*for mem_forward*)
@@ -19,28 +20,27 @@ Require Import Linear.
 Require Import Linear_coop.
 Require Import BuiltinEffects.
 
-Section EFFSEM.
+Section LINEAR_EFF.
+Variable hf : I64Helpers.helper_functions.
 
-Variable ge: genv.
-
-Inductive linear_effstep: (block -> Z -> bool) -> Linear_core -> mem -> Linear_core -> mem -> Prop :=
+Inductive linear_effstep (ge:genv): (block -> Z -> bool) -> Linear_core -> mem -> Linear_core -> mem -> Prop :=
   | lin_effexec_Lgetstack:
       forall s f sp sl ofs ty dst b rs m rs' lf,
       rs' = Locmap.set (R dst) (rs (S sl ofs ty)) (undef_regs (destroyed_by_getstack sl) rs) ->
-      linear_effstep EmptyEffect 
+      linear_effstep ge EmptyEffect 
         (Linear_State s f sp (Lgetstack sl ofs ty dst :: b) rs lf) m
         (Linear_State s f sp b rs' lf) m
   | lin_effexec_Lsetstack:
       forall s f sp src sl ofs ty b rs m rs' lf,
       rs' = Locmap.set (S sl ofs ty) (rs (R src)) (undef_regs (destroyed_by_setstack ty) rs) ->
-      linear_effstep EmptyEffect 
+      linear_effstep ge EmptyEffect 
         (Linear_State s f sp (Lsetstack src sl ofs ty :: b) rs lf) m
         (Linear_State s f sp b rs' lf) m
   | lin_effexec_Lop:
       forall s f sp op args res b rs m v rs' lf,
       eval_operation ge sp op (reglist rs args) m = Some v ->
       rs' = Locmap.set (R res) v (undef_regs (destroyed_by_op op) rs) ->
-      linear_effstep EmptyEffect 
+      linear_effstep ge EmptyEffect 
         (Linear_State s f sp (Lop op args res :: b) rs lf) m
         (Linear_State s f sp b rs' lf) m
   | lin_effexec_Lload:
@@ -48,7 +48,7 @@ Inductive linear_effstep: (block -> Z -> bool) -> Linear_core -> mem -> Linear_c
       eval_addressing ge sp addr (reglist rs args) = Some a ->
       Mem.loadv chunk m a = Some v ->
       rs' = Locmap.set (R dst) v (undef_regs (destroyed_by_load chunk addr) rs) ->
-      linear_effstep EmptyEffect 
+      linear_effstep ge EmptyEffect 
         (Linear_State s f sp (Lload chunk addr args dst :: b) rs lf) m
         (Linear_State s f sp b rs' lf) m
   | lin_effexec_Lstore:
@@ -56,14 +56,14 @@ Inductive linear_effstep: (block -> Z -> bool) -> Linear_core -> mem -> Linear_c
       eval_addressing ge sp addr (reglist rs args) = Some a ->
       Mem.storev chunk m a (rs (R src)) = Some m' ->
       rs' = undef_regs (destroyed_by_store chunk addr) rs ->
-      linear_effstep (StoreEffect a (encode_val chunk (rs (R src))))
+      linear_effstep ge (StoreEffect a (encode_val chunk (rs (R src))))
         (Linear_State s f sp (Lstore chunk addr args src :: b) rs lf) m
         (Linear_State s f sp b rs' lf) m'
   | lin_effexec_Lcall:
       forall s f sp sig ros b rs m f' lf,
       find_function ge ros rs = Some f' ->
       sig = funsig f' ->
-      linear_effstep EmptyEffect 
+      linear_effstep ge EmptyEffect 
         (Linear_State s f sp (Lcall sig ros :: b) rs lf) m
         (Linear_Callstate (Stackframe f sp rs b:: s) f' rs lf) m
   | lin_effexec_Ltailcall:
@@ -73,15 +73,15 @@ Inductive linear_effstep: (block -> Z -> bool) -> Linear_core -> mem -> Linear_c
       find_function ge ros rs' = Some f' ->
       sig = funsig f' ->
       Mem.free m stk 0 f.(fn_stacksize) = Some m' ->
-      linear_effstep (FreeEffect m 0 (f.(fn_stacksize)) stk)
+      linear_effstep ge (FreeEffect m 0 (f.(fn_stacksize)) stk)
         (Linear_State s f (Vptr stk Int.zero) (Ltailcall sig ros :: b) rs lf) m
         (Linear_Callstate s f' rs' lf) m'
   | lin_effexec_Lbuiltin:
       forall s f sp rs m ef args res b t vl rs' m' lf,
       external_call' ef ge (reglist rs args) m t vl m' ->
-      observableEF ef = false ->
+      observableEF hf ef = false ->
       rs' = Locmap.setlist (map R res) vl (undef_regs (destroyed_by_builtin ef) rs) ->
-      linear_effstep (BuiltinEffect ge ef (decode_longs (sig_args (ef_sig ef)) (reglist rs args)) m)
+      linear_effstep ge (BuiltinEffect ge ef (decode_longs (sig_args (ef_sig ef)) (reglist rs args)) m)
          (Linear_State s f sp (Lbuiltin ef args res :: b) rs lf) m
          (Linear_State s f sp b rs' lf) m'
 (*NO ANNOTS YET
@@ -92,13 +92,13 @@ Inductive linear_effstep: (block -> Z -> bool) -> Linear_core -> mem -> Linear_c
          (Linear_State s f sp b rs lf) m'*)
   | lin_effexec_Llabel:
       forall s f sp lbl b rs m lf,
-      linear_effstep EmptyEffect 
+      linear_effstep ge EmptyEffect 
         (Linear_State s f sp (Llabel lbl :: b) rs lf) m
         (Linear_State s f sp b rs lf) m
   | lin_effexec_Lgoto:
       forall s f sp lbl b rs m b' lf,
       find_label lbl f.(fn_code) = Some b' ->
-      linear_effstep EmptyEffect 
+      linear_effstep ge EmptyEffect 
         (Linear_State s f sp (Lgoto lbl :: b) rs lf) m
         (Linear_State s f sp b' rs lf) m
   | lin_effexec_Lcond_true:
@@ -106,14 +106,14 @@ Inductive linear_effstep: (block -> Z -> bool) -> Linear_core -> mem -> Linear_c
       eval_condition cond (reglist rs args) m = Some true ->
       rs' = undef_regs (destroyed_by_cond cond) rs ->
       find_label lbl f.(fn_code) = Some b' ->
-      linear_effstep EmptyEffect 
+      linear_effstep ge EmptyEffect 
         (Linear_State s f sp (Lcond cond args lbl :: b) rs lf) m
         (Linear_State s f sp b' rs' lf) m
   | lin_effexec_Lcond_false:
       forall s f sp cond args lbl b rs m rs' lf,
       eval_condition cond (reglist rs args) m = Some false ->
       rs' = undef_regs (destroyed_by_cond cond) rs ->
-      linear_effstep EmptyEffect 
+      linear_effstep ge EmptyEffect 
         (Linear_State s f sp (Lcond cond args lbl :: b) rs lf) m
         (Linear_State s f sp b rs' lf) m
   | lin_effexec_Ljumptable:
@@ -122,47 +122,48 @@ Inductive linear_effstep: (block -> Z -> bool) -> Linear_core -> mem -> Linear_c
       list_nth_z tbl (Int.unsigned n) = Some lbl ->
       find_label lbl f.(fn_code) = Some b' ->
       rs' = undef_regs (destroyed_by_jumptable) rs ->
-      linear_effstep EmptyEffect 
+      linear_effstep ge EmptyEffect 
         (Linear_State s f sp (Ljumptable arg tbl :: b) rs lf) m
         (Linear_State s f sp b' rs' lf) m
   | lin_effexec_Lreturn:
       forall s f stk b rs m m' rs0 f0,
       let lf := mk_load_frame rs0 f0 in
       Mem.free m stk 0 f.(fn_stacksize) = Some m' ->
-      linear_effstep (FreeEffect m 0 (f.(fn_stacksize)) stk)
+      linear_effstep ge (FreeEffect m 0 (f.(fn_stacksize)) stk)
         (Linear_State s f (Vptr stk Int.zero) (Lreturn :: b) rs lf) m
         (Linear_Returnstate s (sig_res (fn_sig f)) (return_regs (parent_locset0 rs0 s) rs) lf) m'
   | lin_effexec_function_internal0:
       forall s f rs m rs0 f0,
-      linear_effstep EmptyEffect 
+      linear_effstep ge EmptyEffect 
                      (Linear_CallstateIn s (Internal f) rs (mk_load_frame rs0 f0)) m
                      (Linear_Callstate s (Internal f) rs (mk_load_frame (call_regs rs0) f0)) m
   | lin_effexec_function_internal:
       forall s f rs m rs' m' stk lf,
       Mem.alloc m 0 f.(fn_stacksize) = (m', stk) ->
       rs' = undef_regs destroyed_at_function_entry (call_regs rs) ->
-      linear_effstep EmptyEffect 
+      linear_effstep ge EmptyEffect 
         (Linear_Callstate s (Internal f) rs lf) m
         (Linear_State s f (Vptr stk Int.zero) f.(fn_code) rs' lf) m'
-(*NO RULE FOR EXTERNAL CALLS
+
   | lin_effexec_function_external:
-      forall s ef args res rs1 rs2 m t m',
+      forall s ef args res rs1 rs2 m t m' lf
+      (OBS: observableEF hf ef = false),
       args = map rs1 (loc_arguments (ef_sig ef)) ->
       external_call' ef ge args m t res m' ->
       rs2 = Locmap.setlist (map R (loc_result (ef_sig ef))) res rs1 ->
-      linear_effstep (Linear_Callstate s (External ef) rs1) m
-          (Linear_Returnstate s rs2) m'*)
+      linear_effstep ge (BuiltinEffect ge ef args m)
+          (Linear_Callstate s (External ef) rs1 lf) m
+          (Linear_Returnstate s (sig_res (ef_sig ef)) rs2 lf) m'
+
   | lin_effexec_return:
       forall s f sp lf c retty rs m rs_init,
-      linear_effstep EmptyEffect 
+      linear_effstep ge EmptyEffect 
         (Linear_Returnstate (Stackframe f sp lf c :: s) retty rs rs_init) m
         (Linear_State s f sp c rs rs_init) m.
 
-End EFFSEM.
-
 Lemma linearstep_effax1: forall (M : block -> Z -> bool) g c m c' m',
       linear_effstep g M c m c' m' ->
-      (corestep Linear_coop_sem g c m c' m' /\
+      (corestep (Linear_coop_sem hf) g c m c' m' /\
        Mem.unchanged_on (fun (b : block) (ofs : Z) => M b ofs = false) m m').
 Proof. 
 intros.
@@ -206,13 +207,18 @@ intros.
          eapply Mem.unchanged_on_refl.
   split. unfold corestep, coopsem; simpl. econstructor; eassumption.
          eapply Mem.alloc_unchanged_on; eassumption. 
-  (*no external call*) 
+  split. unfold corestep, coopsem; simpl. econstructor; eassumption.
+         inv H0.
+         eapply mem_unchanged_on_sub.
+           eapply BuiltinEffect_unchOn; eassumption. 
+         simpl. unfold BuiltinEffect. intros.
+           destruct ef; trivial. 
   split. unfold corestep, coopsem; simpl. econstructor; eassumption.
          apply Mem.unchanged_on_refl.
 Qed.
 
-Lemma linearstep_effax2: forall  g c m c' m',
-      corestep Linear_coop_sem g c m c' m' ->
+Lemma linearstep_effax2 g c m c' m':
+      corestep (Linear_coop_sem hf) g c m c' m' ->
       exists M, linear_effstep g M c m c' m'.
 Proof.
 intros. unfold corestep, coopsem in H; simpl in H.
@@ -234,6 +240,7 @@ intros. unfold corestep, coopsem in H; simpl in H.
     eexists. eapply lin_effexec_Lreturn; eassumption.
     eexists. eapply lin_effexec_function_internal0; eassumption.
     eexists. eapply lin_effexec_function_internal; try eassumption; trivial.
+    eexists. eapply lin_effexec_function_external; try eassumption; trivial.
     eexists. eapply lin_effexec_return.
 Qed.
 
@@ -252,12 +259,15 @@ intros.
   eapply FreeEffect_validblock; eassumption.
   eapply BuiltinEffect_valid_block; eassumption.
   eapply FreeEffect_validblock; eassumption.
+  eapply BuiltinEffect_valid_block; eassumption.
 Qed.
 
 Program Definition Linear_eff_sem : 
   @EffectSem genv Linear_core.
-eapply Build_EffectSem with (sem := Linear_coop_sem)(effstep:=linear_effstep).
+eapply Build_EffectSem with (sem := Linear_coop_sem hf)(effstep:=linear_effstep).
 apply linearstep_effax1.
 apply linearstep_effax2.
 apply linear_effstep_valid.
 Defined.
+
+End LINEAR_EFF.
