backend/SelectLongproofEFF.v
@@ -30,81 +30,32 @@ Require Import BuiltinEffects.
 (*Require Import mem_lemmas.
 Require Import StructuredInjections.
 Require Import reach.*)
+
+Require Import I64Helpers.
+Require Import BuiltinEffects.
 Require Import SelectLongNEW.
 
 Open Local Scope cminorsel_scope.
 
 (** * Axiomatization of the helper functions *)
 
-Section HELPERS.
-
-Context {F V: Type} (ge: Genv.t (AST.fundef F) V).
-(*
-Definition helper_injects ef vargs vres : Prop :=
-  forall {TF TV:Type} (tge:Genv.t TF TV) (GDE: genvs_domain_eq ge tge) 
-       (SymbPres: forall s, Genv.find_symbol tge s = Genv.find_symbol ge s)
-        m t m1 mu tm vargs'
-       (WD: SM_wd mu) (SMV: sm_valid mu m tm) (RC: REACH_closed m (vis mu)),
-       meminj_preserves_globals ge (as_inj mu) ->
-       external_call ef ge vargs m t vres m1 ->
-       Mem.inject (as_inj mu) m tm ->
-       val_list_inject (restrict (as_inj mu) (vis mu)) vargs vargs' ->
-       exists mu' vres' tm1,
-         external_call ef tge vargs' tm t vres' tm1 /\
-         val_inject (restrict (as_inj mu') (vis mu')) vres vres' /\
-         Mem.inject (as_inj mu') m1 tm1 /\
-         Mem.unchanged_on (loc_unmapped (restrict (as_inj mu) (vis mu))) m m1 /\
-         Mem.unchanged_on (loc_out_of_reach (restrict (as_inj mu) (vis mu)) m) tm tm1 /\
-         intern_incr mu mu' /\
-         sm_inject_separated mu mu' m tm /\
-         sm_locally_allocated mu mu' m tm m1 tm1 /\
-         SM_wd mu' /\ sm_valid mu' m1 tm1 /\
-         (REACH_closed m (vis mu) -> REACH_closed m1 (vis mu')).
-*)
-Definition helper_implements (id: ident) (sg: signature) (vargs: list val) (vres: val) : Prop :=
-  exists b, exists ef,
-     Genv.find_symbol ge id = Some b
-  /\ Genv.find_funct_ptr ge b = Some (External ef)
-  /\ ef_sig ef = sg
-  /\ (forall m, external_call ef ge vargs m E0 vres m)
-  (*NEW*) /\ observableEF ef = false
-  (*NEW /\ helper_injects ef vargs vres*).
-
-Definition builtin_implements (id: ident) (sg: signature) (vargs: list val) (vres: val) : Prop :=
-  forall m, external_call (EF_builtin id sg) ge vargs m E0 vres m.
-
-Definition i64_helpers_correct (*(hf: helper_functions)*) : Prop :=
-    (forall x z, Val.longoffloat x = Some z -> helper_implements hf.(i64_dtos) sig_f_l (x::nil) z)
-  /\(forall x z, Val.longuoffloat x = Some z -> helper_implements hf.(i64_dtou) sig_f_l (x::nil) z)
-  /\(forall x z, Val.floatoflong x = Some z -> helper_implements hf.(i64_stod) sig_l_f (x::nil) z)
-  /\(forall x z, Val.floatoflongu x = Some z -> helper_implements hf.(i64_utod) sig_l_f (x::nil) z)
-  /\(forall x z, Val.singleoflong x = Some z -> helper_implements hf.(i64_stof) sig_l_s (x::nil) z)
-  /\(forall x z, Val.singleoflongu x = Some z -> helper_implements hf.(i64_utof) sig_l_s (x::nil) z)
-  /\(forall x, builtin_implements hf.(i64_neg) sig_l_l (x::nil) (Val.negl x))
-  /\(forall x y, builtin_implements hf.(i64_add) sig_ll_l (x::y::nil) (Val.addl x y))
-  /\(forall x y, builtin_implements hf.(i64_sub) sig_ll_l (x::y::nil) (Val.subl x y))
-  /\(forall x y, builtin_implements hf.(i64_mul) sig_ii_l (x::y::nil) (Val.mull' x y))
-  /\(forall x y z, Val.divls x y = Some z -> helper_implements hf.(i64_sdiv) sig_ll_l (x::y::nil) z)
-  /\(forall x y z, Val.divlu x y = Some z -> helper_implements hf.(i64_udiv) sig_ll_l (x::y::nil) z)
-  /\(forall x y z, Val.modls x y = Some z -> helper_implements hf.(i64_smod) sig_ll_l (x::y::nil) z)
-  /\(forall x y z, Val.modlu x y = Some z -> helper_implements hf.(i64_umod) sig_ll_l (x::y::nil) z)
-  /\(forall x y, helper_implements hf.(i64_shl) sig_li_l (x::y::nil) (Val.shll x y))
-  /\(forall x y, helper_implements hf.(i64_shr) sig_li_l (x::y::nil) (Val.shrlu x y))
-  /\(forall x y, helper_implements hf.(i64_sar) sig_li_l (x::y::nil) (Val.shrl x y)).
-
-End HELPERS.
-
 (** * Correctness of the instruction selection functions for 64-bit operators *)
 
 Section CMCONSTR.
 
-(*Now in builtineffects Variable hf: helper_functions.*)
 Variable ge: genv.
-Hypothesis HELPERS: i64_helpers_correct ge (*hf*).
+Variable hf: helper_functions.
+(*Lemma HELPERS: i64_helpers_correct ge hf.
+  Proof. apply get_helpers_correct. Qed.*)
+Hypothesis HELPERS: i64_helpers_correct ge hf.
 Variable sp: val.
 Variable e: env.
 Variable m: mem.
-
+(*
+Ltac UseHelper :=
+  let x := fresh "x" in generalize HELPERS as x; intro; red in x;
+  repeat (eauto; match goal with | [ H: _ /\ _ |- _ ] => destruct H end).
+*)
 Ltac UseHelper :=
   red in HELPERS;
   repeat (eauto; match goal with | [ H: _ /\ _ |- _ ] => destruct H end).
@@ -112,7 +63,7 @@ Ltac UseHelper :=
 Lemma eval_helper:
   forall le id sg args vargs vres,
   eval_exprlist ge sp e m le args vargs ->
-  helper_implements ge id sg vargs vres ->
+  helper_implements ge hf id sg vargs vres ->
   eval_expr ge sp e m le (Eexternal id sg args) vres.
 Proof.
   intros. destruct H0 as (b & ef & A & B & C & D & E). econstructor; eauto.
@@ -121,7 +72,7 @@ Qed.
 Corollary eval_helper_1:
   forall le id sg arg1 varg1 vres,
   eval_expr ge sp e m le arg1 varg1 ->
-  helper_implements ge id sg (varg1::nil) vres ->
+  helper_implements ge hf id sg (varg1::nil) vres ->
   eval_expr ge sp e m le (Eexternal id sg (arg1 ::: Enil)) vres.
 Proof.
   intros. eapply eval_helper; eauto. constructor; auto. constructor.
@@ -131,7 +82,7 @@ Corollary eval_helper_2:
   forall le id sg arg1 arg2 varg1 varg2 vres,
   eval_expr ge sp e m le arg1 varg1 ->
   eval_expr ge sp e m le arg2 varg2 ->
-  helper_implements ge id sg (varg1::varg2::nil) vres ->
+  helper_implements ge hf id sg (varg1::varg2::nil) vres ->
   eval_expr ge sp e m le (Eexternal id sg (arg1 ::: arg2 ::: Enil)) vres.
 Proof.
   intros. eapply eval_helper; eauto. constructor; auto. constructor; auto. constructor.
@@ -398,7 +349,7 @@ Proof.
   f_equal. destruct (zlt (i0 - Int.zwordsize + (Int.zwordsize - 1)) Int.zwordsize); omega.
 Qed.
 
-Theorem eval_negl: unary_constructor_sound (*(negl hf)*) negl Val.negl.
+Theorem eval_negl: unary_constructor_sound (negl hf) Val.negl.
 Proof.
   unfold negl; red; intros. destruct (is_longconst a) eqn:E.
   econstructor; split. apply eval_longconst.  
@@ -422,7 +373,7 @@ Theorem eval_longoffloat:
   forall le a x y,
   eval_expr ge sp e m le a x ->
   Val.longoffloat x = Some y ->
-  exists v, eval_expr ge sp e m le (longoffloat (*hf*) a) v /\ Val.lessdef y v.
+  exists v, eval_expr ge sp e m le (longoffloat hf a) v /\ Val.lessdef y v.
 Proof.
   intros; unfold longoffloat. econstructor; split. 
   eapply eval_helper_1; eauto. UseHelper. 
@@ -433,7 +384,7 @@ Theorem eval_longuoffloat:
   forall le a x y,
   eval_expr ge sp e m le a x ->
   Val.longuoffloat x = Some y ->
-  exists v, eval_expr ge sp e m le (longuoffloat (*hf*) a) v /\ Val.lessdef y v.
+  exists v, eval_expr ge sp e m le (longuoffloat hf a) v /\ Val.lessdef y v.
 Proof.
   intros; unfold longuoffloat. econstructor; split. 
   eapply eval_helper_1; eauto. UseHelper. 
@@ -444,7 +395,7 @@ Theorem eval_floatoflong:
   forall le a x y,
   eval_expr ge sp e m le a x ->
   Val.floatoflong x = Some y ->
-  exists v, eval_expr ge sp e m le (floatoflong (*hf*) a) v /\ Val.lessdef y v.
+  exists v, eval_expr ge sp e m le (floatoflong hf a) v /\ Val.lessdef y v.
 Proof.
   intros; unfold floatoflong. econstructor; split. 
   eapply eval_helper_1; eauto. UseHelper. 
@@ -455,7 +406,7 @@ Theorem eval_floatoflongu:
   forall le a x y,
   eval_expr ge sp e m le a x ->
   Val.floatoflongu x = Some y ->
-  exists v, eval_expr ge sp e m le (floatoflongu (*hf*) a) v /\ Val.lessdef y v.
+  exists v, eval_expr ge sp e m le (floatoflongu hf a) v /\ Val.lessdef y v.
 Proof.
   intros; unfold floatoflongu. econstructor; split. 
   eapply eval_helper_1; eauto. UseHelper. 
@@ -466,7 +417,7 @@ Theorem eval_singleoflong:
   forall le a x y,
   eval_expr ge sp e m le a x ->
   Val.singleoflong x = Some y ->
-  exists v, eval_expr ge sp e m le (singleoflong (*hf*) a) v /\ Val.lessdef y v.
+  exists v, eval_expr ge sp e m le (singleoflong hf a) v /\ Val.lessdef y v.
 Proof.
   intros; unfold singleoflong. econstructor; split. 
   eapply eval_helper_1; eauto. UseHelper. 
@@ -477,7 +428,7 @@ Theorem eval_singleoflongu:
   forall le a x y,
   eval_expr ge sp e m le a x ->
   Val.singleoflongu x = Some y ->
-  exists v, eval_expr ge sp e m le (singleoflongu (*hf*) a) v /\ Val.lessdef y v.
+  exists v, eval_expr ge sp e m le (singleoflongu hf a) v /\ Val.lessdef y v.
 Proof.
   intros; unfold singleoflongu. econstructor; split. 
   eapply eval_helper_1; eauto. UseHelper. 
@@ -578,7 +529,7 @@ Qed.
 
 Lemma eval_shllimm:
   forall n,
-  unary_constructor_sound (fun e => shllimm (*hf*) e n) (fun v => Val.shll v (Vint n)).
+  unary_constructor_sound (fun e => shllimm hf e n) (fun v => Val.shll v (Vint n)).
 Proof.
   unfold shllimm; red; intros.
   apply eval_shift_imm; intros.
@@ -611,7 +562,7 @@ Proof.
     econstructor; split. eapply eval_helper_2; eauto. EvalOp. UseHelper. auto.
 Qed.
 
-Theorem eval_shll: binary_constructor_sound (shll (*hf*)) Val.shll.
+Theorem eval_shll: binary_constructor_sound (shll hf) Val.shll.
 Proof.
   unfold shll; red; intros.
   destruct (is_intconst b) as [n|] eqn:IC.
@@ -624,7 +575,7 @@ Qed.
 
 Lemma eval_shrluimm:
   forall n,
-  unary_constructor_sound (fun e => shrluimm (*hf*) e n) (fun v => Val.shrlu v (Vint n)).
+  unary_constructor_sound (fun e => shrluimm hf e n) (fun v => Val.shrlu v (Vint n)).
 Proof.
   unfold shrluimm; red; intros. apply eval_shift_imm; intros.
   + (* n = 0 *)
@@ -656,7 +607,7 @@ Proof.
     econstructor; split. eapply eval_helper_2; eauto. EvalOp. UseHelper. auto.
 Qed.
 
-Theorem eval_shrlu: binary_constructor_sound (shrlu (*hf*)) Val.shrlu.
+Theorem eval_shrlu: binary_constructor_sound (shrlu hf) Val.shrlu.
 Proof.
   unfold shrlu; red; intros.
   destruct (is_intconst b) as [n|] eqn:IC.
@@ -669,7 +620,7 @@ Qed.
 
 Lemma eval_shrlimm:
   forall n,
-  unary_constructor_sound (fun e => shrlimm (*hf*) e n) (fun v => Val.shrl v (Vint n)).
+  unary_constructor_sound (fun e => shrlimm hf e n) (fun v => Val.shrl v (Vint n)).
 Proof.
   unfold shrlimm; red; intros. apply eval_shift_imm; intros.
   + (* n = 0 *)
@@ -705,7 +656,7 @@ Proof.
     econstructor; split. eapply eval_helper_2; eauto. EvalOp. UseHelper. auto.
 Qed.
 
-Theorem eval_shrl: binary_constructor_sound (shrl (*hf*)) Val.shrl.
+Theorem eval_shrl: binary_constructor_sound (shrl hf) Val.shrl.
 Proof.
   unfold shrl; red; intros.
   destruct (is_intconst b) as [n|] eqn:IC.
@@ -716,7 +667,7 @@ Proof.
   econstructor; split. eapply eval_helper_2; eauto. UseHelper. auto.
 Qed.
 
-Theorem eval_addl: binary_constructor_sound (addl (*hf*)) Val.addl.
+Theorem eval_addl: binary_constructor_sound (addl hf) Val.addl.
 Proof.
   unfold addl; red; intros.
   set (default := Ebuiltin (EF_builtin (i64_add hf) sig_ll_l) (a ::: b ::: Enil)).
@@ -739,7 +690,7 @@ Proof.
 - auto.
 Qed.
 
-Theorem eval_subl: binary_constructor_sound (subl (*hf*)) Val.subl.
+Theorem eval_subl: binary_constructor_sound (subl hf) Val.subl.
 Proof.
   unfold subl; red; intros.
   set (default := Ebuiltin (EF_builtin (i64_sub hf) sig_ll_l) (a ::: b ::: Enil)).
@@ -763,7 +714,7 @@ Proof.
 - auto.
 Qed.
 
-Lemma eval_mull_base: binary_constructor_sound (mull_base (*hf*)) Val.mull.
+Lemma eval_mull_base: binary_constructor_sound (mull_base hf) Val.mull.
 Proof.
   unfold mull_base; red; intros. apply eval_splitlong2; auto.
 - intros. 
@@ -785,7 +736,7 @@ Proof.
 Qed.
 
 Lemma eval_mullimm:
-  forall n, unary_constructor_sound (fun a => mullimm (*hf*) a n) (fun v => Val.mull v (Vlong n)).
+  forall n, unary_constructor_sound (fun a => mullimm hf a n) (fun v => Val.mull v (Vlong n)).
 Proof.
   unfold mullimm; red; intros.
   predSpec Int64.eq Int64.eq_spec n Int64.zero.
@@ -815,7 +766,7 @@ Proof.
   apply eval_mull_base; auto. apply eval_longconst. 
 Qed.
 
-Theorem eval_mull: binary_constructor_sound (mull (*hf*)) Val.mull.
+Theorem eval_mull: binary_constructor_sound (mull hf) Val.mull.
 Proof.
   unfold mull; red; intros.
   destruct (is_longconst a) as [p|] eqn:LC1;
@@ -835,7 +786,7 @@ Qed.
 Lemma eval_binop_long:
   forall id sem le a b x y z,
   (forall p q, x = Vlong p -> y = Vlong q -> z = Vlong (sem p q)) ->
-  helper_implements ge id sig_ll_l (x::y::nil) z ->
+  helper_implements ge hf id sig_ll_l (x::y::nil) z ->
   eval_expr ge sp e m le a x ->
   eval_expr ge sp e m le b y ->
   exists v, eval_expr ge sp e m le (binop_long id sem a b) v /\ Val.lessdef z v.
@@ -855,7 +806,7 @@ Theorem eval_divl:
   eval_expr ge sp e m le a x ->
   eval_expr ge sp e m le b y ->
   Val.divls x y = Some z ->
-  exists v, eval_expr ge sp e m le (divl (*hf*) a b) v /\ Val.lessdef z v.
+  exists v, eval_expr ge sp e m le (divl hf a b) v /\ Val.lessdef z v.
 Proof.
   intros. eapply eval_binop_long; eauto. 
   intros; subst; simpl in H1.
@@ -870,7 +821,7 @@ Theorem eval_modl:
   eval_expr ge sp e m le a x ->
   eval_expr ge sp e m le b y ->
   Val.modls x y = Some z ->
-  exists v, eval_expr ge sp e m le (modl (*hf*) a b) v /\ Val.lessdef z v.
+  exists v, eval_expr ge sp e m le (modl hf a b) v /\ Val.lessdef z v.
 Proof.
   intros. eapply eval_binop_long; eauto. 
   intros; subst; simpl in H1.
@@ -885,7 +836,7 @@ Theorem eval_divlu:
   eval_expr ge sp e m le a x ->
   eval_expr ge sp e m le b y ->
   Val.divlu x y = Some z ->
-  exists v, eval_expr ge sp e m le (divlu (*hf*) a b) v /\ Val.lessdef z v.
+  exists v, eval_expr ge sp e m le (divlu hf a b) v /\ Val.lessdef z v.
 Proof.
   intros. unfold divlu. 
   set (default := Eexternal (i64_udiv hf) sig_ll_l (a ::: b ::: Enil)).
@@ -928,7 +879,7 @@ Theorem eval_modlu:
   eval_expr ge sp e m le a x ->
   eval_expr ge sp e m le b y ->
   Val.modlu x y = Some z ->
-  exists v, eval_expr ge sp e m le (modlu (*hf*) a b) v /\ Val.lessdef z v.
+  exists v, eval_expr ge sp e m le (modlu hf a b) v /\ Val.lessdef z v.
 Proof.
   intros. unfold modlu. 
   set (default := Eexternal (i64_umod hf) sig_ll_l (a ::: b ::: Enil)).
