backend/LinearizeproofEFF.v
@@ -66,6 +66,8 @@ Hypothesis TRANSF: transf_program prog = OK tprog.
 Let ge := Genv.globalenv prog.
 Let tge := Genv.globalenv tprog.
 
+(*NEW*) Variable hf : I64Helpers.helper_functions.
+
 Lemma functions_translated:
   forall v f,
   Genv.find_funct ge v = Some f ->
@@ -278,7 +280,7 @@ Lemma starts_with_correct:
   unique_labels c2 ->
   starts_with lbl c1 = true ->
   find_label lbl c2 = Some c3 ->
-  corestep_plus Linear_eff_sem tge
+  corestep_plus (Linear_eff_sem hf) tge
               (Linear_State s f sp c1 ls ls0) m
               (Linear_State s f sp c3 ls ls0) m.
 Proof.
@@ -303,7 +305,7 @@ Lemma starts_with_correct_eff:
   unique_labels c2 ->
   starts_with lbl c1 = true ->
   find_label lbl c2 = Some c3 ->
-  effstep_plus Linear_eff_sem tge EmptyEffect
+  effstep_plus (Linear_eff_sem hf) tge EmptyEffect
               (Linear_State s f sp c1 ls ls0) m
               (Linear_State s f sp c3 ls ls0) m.
 Proof.
@@ -511,7 +513,7 @@ Lemma add_branch_correct:
   transf_function f = OK tf ->
   is_tail k tf.(fn_code) ->
   find_label lbl tf.(fn_code) = Some c ->
-  corestep_plus Linear_eff_sem tge
+  corestep_plus (Linear_eff_sem hf) tge
                (Linear_State s tf sp (add_branch lbl k) ls ls0) m
                (Linear_State s tf sp c ls ls0) m.
 Proof.
@@ -527,7 +529,7 @@ Lemma add_branch_correct_eff:
   transf_function f = OK tf ->
   is_tail k tf.(fn_code) ->
   find_label lbl tf.(fn_code) = Some c ->
-  effstep_plus Linear_eff_sem tge EmptyEffect
+  effstep_plus (Linear_eff_sem hf) tge EmptyEffect
                (Linear_State s tf sp (add_branch lbl k) ls ls0) m
                (Linear_State s tf sp c ls ls0) m.
 Proof.
@@ -1037,11 +1039,11 @@ Qed.
 
 Lemma MATCH_atExternal: forall mu c1 m1 c2 m2 e vals1 ef_sig
        (MTCH: MATCH mu c1 m1 c2 m2)
-       (AtExtSrc: at_external LTL_eff_sem c1 = Some (e, ef_sig, vals1)),
+       (AtExtSrc: at_external (LTL_eff_sem hf) c1 = Some (e, ef_sig, vals1)),
      Mem.inject (as_inj mu) m1 m2 /\
      exists vals2,
        Forall2 (val_inject (restrict (as_inj mu) (vis mu))) vals1 vals2 /\
-       at_external Linear_eff_sem c2 = Some (e, ef_sig, vals2) /\
+       at_external (Linear_eff_sem hf) c2 = Some (e, ef_sig, vals2) /\
       (forall pubSrc' pubTgt',
        pubSrc' = (fun b => locBlocksSrc mu b && REACH m1 (exportedSrc mu vals1) b) ->
        pubTgt' = (fun b : block => locBlocksTgt mu b && REACH m2 (exportedTgt mu vals2) b) ->
@@ -1053,7 +1055,7 @@ inv MC; simpl in AtExtSrc; inv AtExtSrc.
 destruct f; try inv H1. inv H3.
 destruct f; simpl in *; inv H2.
 split; trivial. monadInv H0.
-destruct (observableEF e0); inv H3.
+destruct (observableEF hf e0); inv H3.
 assert (ValsInj: Forall2 (val_inject (restrict (as_inj mu) (vis mu)))
   (decode_longs (sig_args (ef_sig e)) (ls1 ## (Conventions1.loc_arguments (ef_sig e))))
   (decode_longs (sig_args (ef_sig e)) (ls2 ## (Conventions1.loc_arguments (ef_sig e))))).
@@ -1223,8 +1225,8 @@ Lemma MATCH_afterExternal: forall
       mu st1 st2 m1 e vals1 m2 ef_sig vals2 e' ef_sig'
       (MemInjMu : Mem.inject (as_inj mu) m1 m2)
       (MatchMu: MATCH mu st1 m1 st2 m2)
-      (AtExtSrc : at_external LTL_eff_sem st1 = Some (e, ef_sig, vals1))
-      (AtExtTgt : at_external Linear_eff_sem st2 = Some (e', ef_sig', vals2))
+      (AtExtSrc : at_external (LTL_eff_sem hf) st1 = Some (e, ef_sig, vals1))
+      (AtExtTgt : at_external (Linear_eff_sem hf) st2 = Some (e', ef_sig', vals2))
       (ValInjMu : Forall2 (val_inject (restrict (as_inj mu) (vis mu))) vals1 vals2)
       (pubSrc' : block -> bool)
       (pubSrcHyp : pubSrc' =
@@ -1257,8 +1259,8 @@ Lemma MATCH_afterExternal: forall
                (fun b z => locBlocksSrc nu b = true /\ pubBlocksSrc nu b = false) m1 m1')
        (UnchLOOR: Mem.unchanged_on (local_out_of_reach nu m1) m2 m2'),
   exists st1' st2',
-  after_external LTL_eff_sem (Some ret1) st1 =Some st1' /\
-  after_external Linear_eff_sem (Some ret2) st2 = Some st2' /\
+  after_external (LTL_eff_sem hf) (Some ret1) st1 =Some st1' /\
+  after_external (Linear_eff_sem hf) (Some ret2) st2 = Some st2' /\
   MATCH mu' st1' m1' st2' m2'.
 Proof. intros.
 simpl.
@@ -1268,7 +1270,7 @@ simpl.
  destruct f; inv H2. 
  destruct tf; inv AtExtTgt.
  inv H0.
- destruct (observableEF e1); inv H2; inv H3.
+ destruct (observableEF hf e1); inv H2; inv H3.
  eexists. eexists.
     split. reflexivity.
     split. reflexivity.
@@ -1514,7 +1516,7 @@ Lemma MATCH_initial: forall (v1 v2 : val) (sig : signature) entrypoints
                     Genv.find_funct_ptr tge b = Some f2)
   (vals1 : list val) c1 (m1 : mem) (j : meminj)
   (vals2 : list val) (m2 : mem) (DomS DomT : Values.block -> bool)
-  (Ini : initial_core LTL_eff_sem ge v1 vals1 = Some c1)
+  (Ini : initial_core (LTL_eff_sem hf) ge v1 vals1 = Some c1)
   (Inj: Mem.inject j m1 m2)
   (VInj: Forall2 (val_inject j) vals1 vals2)
   (PG: meminj_preserves_globals ge j)
@@ -1531,7 +1533,7 @@ Lemma MATCH_initial: forall (v1 v2 : val) (sig : signature) entrypoints
   (HDomS: forall b : Values.block, DomS b = true -> Mem.valid_block m1 b)
   (HDomT: forall b : Values.block, DomT b = true -> Mem.valid_block m2 b),
 exists c2,
-  initial_core Linear_eff_sem tge v2 vals2 = Some c2 /\
+  initial_core (Linear_eff_sem hf) tge v2 vals2 = Some c2 /\
   MATCH 
     (initial_SM DomS DomT
        (REACH m1
@@ -1624,12 +1626,12 @@ Proof. intros.
 Qed.
 
 Lemma MATCH_corediagram: forall st1 m1 st1' m1'
-         (CS:corestep LTL_eff_sem ge st1 m1 st1' m1')
+         (CS:corestep (LTL_eff_sem hf) ge st1 m1 st1' m1')
          st2 mu m2 (MTCH:MATCH mu st1 m1 st2 m2),
 exists st2' m2', 
-  (corestep_plus Linear_eff_sem tge st2 m2 st2' m2' \/
+  (corestep_plus (Linear_eff_sem hf) tge st2 m2 st2' m2' \/
    (measure st1' < measure st1)%nat /\
-   corestep_star Linear_eff_sem tge st2 m2 st2' m2')
+   corestep_star (Linear_eff_sem hf) tge st2 m2 st2' m2')
 /\ exists mu',
   intern_incr mu mu' /\
   sm_inject_separated mu mu' m1 m2 /\
@@ -1648,7 +1650,7 @@ Proof. intros.
     rewrite varinfo_preserved. intuition.
   induction CS; intros; try (inv MS).
 
-  (* start of block, at an [add_branch] *)
+{ (* start of block, at an [add_branch] *)
   exploit find_label_lin; eauto. intros [k F]. 
   eexists; eexists; split. 
     left. eapply add_branch_correct; eauto.
@@ -1664,9 +1666,9 @@ Proof. intros.
   split; intuition. 
     econstructor; eauto. 
     intros; eapply reachable_successors; eauto.
-    eapply is_tail_lin_block; eauto. eapply is_tail_find_label; eauto.
+    eapply is_tail_lin_block; eauto. eapply is_tail_find_label; eauto. }
 
-  (* start of block, target of an [Lcond] *)
+{ (* start of block, target of an [Lcond] *)
   exploit find_label_lin; eauto. intros [k F]. 
   eexists; eexists; split. 
     left. apply corestep_plus_one. eapply lin_exec_Lcond_true; eauto. 
@@ -1688,9 +1690,9 @@ Proof. intros.
   split; intuition. 
   econstructor; eauto. 
   intros; eapply reachable_successors; eauto.
-  eapply is_tail_lin_block; eauto. eapply is_tail_find_label; eauto.
+  eapply is_tail_lin_block; eauto. eapply is_tail_find_label; eauto. }
 
-  (* start of block, target of an [Ljumptable] *)
+{ (* start of block, target of an [Ljumptable] *)
   exploit find_label_lin; eauto. intros [k F].
   eexists; eexists; split.
   left. apply corestep_plus_one.
@@ -1711,9 +1713,9 @@ Proof. intros.
   split; intuition. 
   econstructor; eauto. 
   intros; eapply reachable_successors; eauto.
-  eapply is_tail_lin_block; eauto. eapply is_tail_find_label; eauto.
+  eapply is_tail_lin_block; eauto. eapply is_tail_find_label; eauto. }
 
-  (* Lop *)
+{ (* Lop *)
   rewrite vis_restrict_sm, restrict_sm_all, restrict_nest in AGREE; trivial.
   exploit (eval_operation_inject'' _ _ ge (as_inj (restrict_sm mu (vis mu)))).
     eapply val_inject_incr; try eapply SPLocal. 
@@ -1743,9 +1745,9 @@ Proof. intros.
   rewrite vis_restrict_sm, restrict_sm_all, restrict_nest; trivial.
     rewrite restrict_sm_all in VINJ.
     eapply agree_regs_set; try eassumption.
-    eapply agree_regs_undef; eassumption.
+    eapply agree_regs_undef; eassumption. }
 
-  (* Lload *)
+{ (* Lload *)
   rewrite vis_restrict_sm, restrict_sm_all, restrict_nest in AGREE; trivial.
   assert (WDR: SM_wd (restrict_sm mu (vis mu))).
    apply restrict_sm_WD; try eassumption. trivial.
@@ -1785,9 +1787,9 @@ Proof. intros.
   econstructor; eauto.
   rewrite vis_restrict_sm, restrict_sm_all, restrict_nest; trivial.
     rewrite restrict_sm_all in D.
-    eapply agree_regs_set; try eassumption.
+    eapply agree_regs_set; try eassumption. }
 
-  (* Lgetstack *)
+{ (* Lgetstack *)
   rewrite vis_restrict_sm, restrict_sm_all, restrict_nest in AGREE; trivial.
   eexists; eexists; split. 
     left. apply corestep_plus_one. econstructor; eauto.
@@ -1805,9 +1807,9 @@ Proof. intros.
   rewrite vis_restrict_sm, restrict_sm_all, restrict_nest; trivial.
   eapply agree_regs_set; try eassumption.
     eapply agree_regs_undef; eassumption. 
-    simpl. eapply AGREE.
+    simpl. eapply AGREE. }
 
-  (* Lsetstack *)
+{ (* Lsetstack *)
   rewrite vis_restrict_sm, restrict_sm_all, restrict_nest in AGREE; trivial.
   eexists; eexists; split. 
     left. apply corestep_plus_one. econstructor; eauto. 
@@ -1823,9 +1825,9 @@ Proof. intros.
   split; intuition. 
   econstructor; eauto.
   rewrite vis_restrict_sm, restrict_sm_all, restrict_nest; trivial.
-    eapply agree_regs_setstack; eassumption.
+    eapply agree_regs_setstack; eassumption. }
 
-  (* Lstore *)
+{ (* Lstore *)
   rewrite vis_restrict_sm, restrict_sm_all, restrict_nest in AGREE; trivial.
   assert (WDR: SM_wd (restrict_sm mu (vis mu))).
    apply restrict_sm_WD; try eassumption. trivial.
@@ -1880,9 +1882,9 @@ Proof. intros.
                   destruct AGREE as [AGREE_R AGREE_S].
                   specialize (AGREE_R src). 
                    rewrite H4 in AGREE_R; inv AGREE_R.   
-                   destruct (restrictD_Some _ _ _ _ _ H8); trivial.
+                   destruct (restrictD_Some _ _ _ _ _ H8); trivial. }
 
-  (* Lcall *)
+{ (* Lcall *)
   rewrite vis_restrict_sm, restrict_sm_all, restrict_nest in AGREE; trivial.
   exploit agree_find_function_translated; try eassumption.
     eapply agree_regs_incr; try eapply AGREE. apply restrict_incr. 
@@ -1902,9 +1904,9 @@ Proof. intros.
   split; intuition. fold linearize_block.
   econstructor; eauto. constructor; auto. econstructor; eauto.
     rewrite vis_restrict_sm, restrict_sm_all, restrict_nest; trivial.
-    rewrite vis_restrict_sm, restrict_sm_all, restrict_nest; trivial.
+    rewrite vis_restrict_sm, restrict_sm_all, restrict_nest; trivial. }
 
-  (* Ltailcall *)
+{ (* Ltailcall *)
   rewrite vis_restrict_sm, restrict_sm_all, restrict_nest in AGREE; trivial.
   destruct ls0; simpl.
   specialize (match_parent_locset0 _ _ rs0 _ STACKS); intros parentsAGREE.
@@ -1943,9 +1945,9 @@ Proof. intros.
   split. econstructor; eauto.
            rewrite vis_restrict_sm, restrict_sm_all, restrict_nest; trivial.
   intuition.
-      eapply REACH_closed_free; try eassumption.
+      eapply REACH_closed_free; try eassumption. }
 
-  (* Lbuiltin*) 
+{ (* Lbuiltin*) 
   inv H. 
   assert (ArgsInj: val_list_inject (restrict (as_inj mu) (vis mu))
             (decode_longs (sig_args (ef_sig ef)) (reglist rs args))
@@ -1986,7 +1988,7 @@ Proof. intros.
           split; trivial.
           eapply intern_incr_as_inj; eassumption.
     assert (FRG: frgnBlocksSrc mu = frgnBlocksSrc mu') by eapply INC.
-          rewrite <- FRG. eapply (Glob _ H2).
+          rewrite <- FRG. eapply (Glob _ H2). }
 
   (* Lannot 
   eexists; eexists; split. 
@@ -1996,7 +1998,7 @@ Proof. intros.
   exact symbols_preserved. exact varinfo_preserved.
   econstructor; eauto.*)
 
-  (* Lbranch *)
+{ (* Lbranch *)
   eexists; eexists; split. 
   assert ((reachable f)!!pc = true). apply REACH; simpl; auto.
   right; split. simpl; omega. eapply corestep_star_zero.
@@ -2009,9 +2011,9 @@ Proof. intros.
       apply extensionality; intros; rewrite (freshloc_irrefl). intuition.
       apply extensionality; intros; rewrite (freshloc_irrefl). intuition.
       apply extensionality; intros; rewrite (freshloc_irrefl). intuition.
-  split; intuition. econstructor; eauto. apply REACH. left. trivial. 
+  split; intuition. econstructor; eauto. apply REACH. left. trivial. }
 
-  (* Lcond *)
+{ (* Lcond *)
   rewrite vis_restrict_sm, restrict_sm_all, restrict_nest in AGREE; trivial.
   exploit eval_condition_inject; try eassumption.
     eapply agree_regs_list; try eassumption.
@@ -2088,8 +2090,9 @@ Proof. intros.
         apply extensionality; intros; rewrite (freshloc_irrefl). intuition.
     split; intuition.
       econstructor; eauto.
-      rewrite vis_restrict_sm, restrict_sm_all, restrict_nest; trivial.
-  (* Ljumptable *)
+      rewrite vis_restrict_sm, restrict_sm_all, restrict_nest; trivial. }
+
+{ (* Ljumptable *)
   assert (REACH': (reachable f)!!pc = true).
     apply REACH. simpl. eapply list_nth_z_in; eauto. 
   eexists; eexists; split.
@@ -2103,9 +2106,9 @@ Proof. intros.
         apply extensionality; intros; rewrite (freshloc_irrefl). intuition.
         apply extensionality; intros; rewrite (freshloc_irrefl). intuition.
         apply extensionality; intros; rewrite (freshloc_irrefl). intuition.
-    split; intuition. econstructor; eauto.
+    split; intuition. econstructor; eauto. }
 
-  (* Lreturn *)
+{ (* Lreturn *)
   destruct ls0.
   rewrite vis_restrict_sm, restrict_sm_all, restrict_nest in AGREE; trivial.
   assert (WDR: SM_wd (restrict_sm mu (vis mu))).
@@ -2120,7 +2123,7 @@ Proof. intros.
            (return_regs (parent_locset0 rs0 ts) ls2) (mk_load_frame rs0 f0)).
   exists tm'; split.
   left. apply corestep_plus_one. 
-    apply (lin_exec_Lreturn tge ts tf spb c ls2 m2 tm' rs0 f0); auto.
+    apply (lin_exec_Lreturn hf tge ts tf spb c ls2 m2 tm' rs0 f0); auto.
     rewrite (stacksize_preserved _ _ TRF). eauto.
   assert (SMV': sm_valid mu m' tm').
     split; intros;  
@@ -2144,9 +2147,9 @@ Proof. intros.
              rewrite vis_restrict_sm, restrict_sm_all, restrict_nest; trivial.
              solve[apply (match_parent_locset0 _ _ _ _ STACKS)].
   intuition.
-      eapply REACH_closed_free; try eassumption.
+      eapply REACH_closed_free; try eassumption. }
 
-  (* dummy step *)
+{ (* dummy step *)
   destruct ls0.
   assert (REACH: (reachable f)!!(LTL.fn_entrypoint f) = true).
     apply reachable_entrypoint.
@@ -2203,9 +2206,9 @@ Proof. intros.
     red; intros. destruct (GFP _ _ H1). split; trivial.
          eapply intern_incr_as_inj; eassumption.
     assert (FF: frgnBlocksSrc mu = frgnBlocksSrc mu') by eapply IntInc.
-      apply Glob in H1. rewrite <-FF; trivial.
+      apply Glob in H1. rewrite <-FF; trivial. }
 
-  (* internal functions *)
+{ (* internal functions *)
   assert (REACH: (reachable f)!!(LTL.fn_entrypoint f) = true).
     apply reachable_entrypoint.
   monadInv H8.
@@ -2259,11 +2262,51 @@ Proof. intros.
     red; intros. destruct (GFP _ _ H1). split; trivial.
          eapply intern_incr_as_inj; eassumption.
     assert (FF: frgnBlocksSrc mu = frgnBlocksSrc mu') by eapply IntInc.
-      apply Glob in H1. rewrite <-FF; trivial.
+      apply Glob in H1. rewrite <-FF; trivial. }
 
-  (* no external function *)
+{ contradiction. }
+{  (* unobservable external function *)
+  monadInv H9. inv H0.
+  rewrite vis_restrict_sm, restrict_sm_all in AGREE.
+  rewrite restrict_nest in AGREE; trivial.
+  assert (ArgsInj: val_list_inject (restrict (as_inj mu) (vis mu))
+            (decode_longs (sig_args (ef_sig ef)) (rs ## (Conventions1.loc_arguments (ef_sig ef))))
+            (decode_longs (sig_args (ef_sig ef)) (ls2 ## (Conventions1.loc_arguments (ef_sig ef))))).
+    simpl. eapply decode_longs_inject. 
+     eapply agree_regs_map_outgoing. assumption.
+     red; intros. apply Conventions1.loc_arguments_rec_charact in H0. 
+           destruct l; try contradiction.
+           destruct sl; try contradiction. trivial.
+  exploit (inlineable_extern_inject ge tge); try eassumption.
+  intros [mu' [v' [m'' [TEC [ResInj [MINJ' [UNMAPPED 
+         [LOOR [INC [SEP [LOCALLOC [WD' [SMV' RC']]]]]]]]]]]]].  
+  eexists; eexists m''.
+  split. left. apply corestep_plus_one. 
+          eapply lin_exec_function_external; eauto.
+          econstructor; eauto.
+  exists mu'. intuition.
+  split.
+    econstructor; eauto.
+     eapply list_match_stackframes_intern_incr; try eassumption.
+       apply restrict_sm_intern_incr; eassumption.
+     eapply restrict_sm_WD; trivial.
+     rewrite vis_restrict_sm, restrict_sm_all; trivial.
+       rewrite restrict_nest; trivial.
+       eapply agree_regs_set_regs; try eassumption.
+       eapply agree_regs_incr; try eassumption.
+         eapply intern_incr_restrict; eassumption.
+       eapply encode_long_inject; eassumption.
+   intuition.
+   apply intern_incr_as_inj in INC; trivial.
+        apply sm_inject_separated_mem in SEP; trivial.
+        eapply meminj_preserves_incr_sep; eassumption. 
+    red; intros ? ? Hb. destruct (GFP _ _ Hb).
+          split; trivial.
+          eapply intern_incr_as_inj; eassumption.
+    assert (FRG: frgnBlocksSrc mu = frgnBlocksSrc mu') by eapply INC.
+          rewrite <- FRG. eapply (Glob _ H1). }
 
-  (* return *) 
+{ (* return *) 
   inv H5. inv H1.
   eexists; eexists; split.
   left. apply corestep_plus_one. econstructor.
@@ -2275,17 +2318,17 @@ Proof. intros.
       repeat split; extensionality b; 
           try rewrite (freshloc_irrefl); intuition.
       split. econstructor; eauto.
-    intuition.
+    intuition. }
 Qed.
 
 Lemma MATCH_effcorediagram: forall st1 m1 st1' m1' (U1 : block -> Z -> bool)
-       (CS:effstep LTL_eff_sem ge U1 st1 m1 st1' m1')
+       (CS:effstep (LTL_eff_sem hf) ge U1 st1 m1 st1' m1')
        st2 mu m2 (U1Vis: forall b ofs, U1 b ofs = true -> vis mu b = true)
        (MTCH: MATCH mu st1 m1 st2 m2),
 exists st2' m2' (U2 : block -> Z -> bool),
-     (effstep_plus Linear_eff_sem tge U2 st2 m2 st2' m2' \/
+     (effstep_plus (Linear_eff_sem hf) tge U2 st2 m2 st2' m2' \/
       (measure st1' < measure st1)%nat /\
-      effstep_star Linear_eff_sem tge U2 st2 m2 st2' m2') 
+      effstep_star (Linear_eff_sem hf) tge U2 st2 m2 st2' m2') 
 /\ exists mu',
   intern_incr mu mu' /\
   sm_inject_separated mu mu' m1 m2 /\
@@ -2312,7 +2355,7 @@ Proof. intros.
     rewrite varinfo_preserved. intuition.
   induction CS; intros; try (inv MS).
 
-  (* start of block, at an [add_branch] *)
+{ (* start of block, at an [add_branch] *)
   exploit find_label_lin; eauto. intros [k F]. 
   eexists; eexists; eexists; split. 
     left. eapply add_branch_correct_eff; eauto.
@@ -2329,9 +2372,9 @@ Proof. intros.
   split; intuition. 
     econstructor; eauto. 
     intros; eapply reachable_successors; eauto.
-    eapply is_tail_lin_block; eauto. eapply is_tail_find_label; eauto.
+    eapply is_tail_lin_block; eauto. eapply is_tail_find_label; eauto. }
 
-  (* start of block, target of an [Lcond] *)
+{ (* start of block, target of an [Lcond] *)
   exploit find_label_lin; eauto. intros [k F]. 
   eexists; eexists; eexists; split. 
     left. apply effstep_plus_one. eapply lin_effexec_Lcond_true; eauto. 
@@ -2354,9 +2397,9 @@ Proof. intros.
   split; intuition. 
   econstructor; eauto. 
   intros; eapply reachable_successors; eauto.
-  eapply is_tail_lin_block; eauto. eapply is_tail_find_label; eauto.
+  eapply is_tail_lin_block; eauto. eapply is_tail_find_label; eauto. }
 
-  (* start of block, target of an [Ljumptable] *)
+{ (* start of block, target of an [Ljumptable] *)
   exploit find_label_lin; eauto. intros [k F].
   eexists; eexists; eexists; split.
   left. apply effstep_plus_one.
@@ -2377,9 +2420,9 @@ Proof. intros.
   split; intuition. 
   econstructor; eauto. 
   intros; eapply reachable_successors; eauto.
-  eapply is_tail_lin_block; eauto. eapply is_tail_find_label; eauto.
+  eapply is_tail_lin_block; eauto. eapply is_tail_find_label; eauto. }
 
-  (* Lop *)
+{ (* Lop *)
   rewrite vis_restrict_sm, restrict_sm_all, restrict_nest in AGREE; trivial.
   exploit (eval_operation_inject'' _ _ ge (as_inj (restrict_sm mu (vis mu)))).
     eapply val_inject_incr; try eapply SPLocal. 
@@ -2410,9 +2453,9 @@ Proof. intros.
   rewrite vis_restrict_sm, restrict_sm_all, restrict_nest; trivial.
     rewrite restrict_sm_all in VINJ.
     eapply agree_regs_set; try eassumption.
-    eapply agree_regs_undef; eassumption.
+    eapply agree_regs_undef; eassumption. }
 
-  (* Lload *)
+{ (* Lload *)
   rewrite vis_restrict_sm, restrict_sm_all, restrict_nest in AGREE; trivial.
   assert (WDR: SM_wd (restrict_sm mu (vis mu))).
    apply restrict_sm_WD; try eassumption. trivial.
@@ -2452,9 +2495,9 @@ Proof. intros.
   econstructor; eauto.
   rewrite vis_restrict_sm, restrict_sm_all, restrict_nest; trivial.
     rewrite restrict_sm_all in D.
-    eapply agree_regs_set; try eassumption.
+    eapply agree_regs_set; try eassumption. }
 
-  (* Lgetstack *)
+{ (* Lgetstack *)
   rewrite vis_restrict_sm, restrict_sm_all, restrict_nest in AGREE; trivial.
   eexists; eexists; eexists; split. 
     left. apply effstep_plus_one. econstructor; eauto.
@@ -2473,9 +2516,9 @@ Proof. intros.
   rewrite vis_restrict_sm, restrict_sm_all, restrict_nest; trivial.
   eapply agree_regs_set; try eassumption.
     eapply agree_regs_undef; eassumption. 
-    simpl. eapply AGREE.
+    simpl. eapply AGREE. }
 
-  (* Lsetstack *)
+{ (* Lsetstack *)
   rewrite vis_restrict_sm, restrict_sm_all, restrict_nest in AGREE; trivial.
   eexists; eexists; eexists; split. 
     left. apply effstep_plus_one. econstructor; eauto. 
@@ -2492,9 +2535,9 @@ Proof. intros.
   split; intuition. 
   econstructor; eauto.
   rewrite vis_restrict_sm, restrict_sm_all, restrict_nest; trivial.
-    eapply agree_regs_setstack; eassumption.
+    eapply agree_regs_setstack; eassumption. }
 
-  (* Lstore *)
+{ (* Lstore *)
   rewrite vis_restrict_sm, restrict_sm_all, restrict_nest in AGREE; trivial.
   assert (WDR: SM_wd (restrict_sm mu (vis mu))).
    apply restrict_sm_WD; try eassumption. trivial.
@@ -2555,9 +2598,9 @@ Proof. intros.
             eapply visPropagateR; eassumption.
     eapply StoreEffect_PropagateLeft; try eassumption.
      econstructor. eassumption. trivial.
-     apply C.
+     apply C. }
     
-  (* Lcall *)
+{ (* Lcall *)
   rewrite vis_restrict_sm, restrict_sm_all, restrict_nest in AGREE; trivial.
   exploit agree_find_function_translated; try eassumption.
     eapply agree_regs_incr; try eapply AGREE. apply restrict_incr. 
@@ -2578,9 +2621,9 @@ Proof. intros.
   split; intuition.
   econstructor; eauto. constructor; auto. econstructor; eauto.
     rewrite vis_restrict_sm, restrict_sm_all, restrict_nest; trivial.
-    rewrite vis_restrict_sm, restrict_sm_all, restrict_nest; trivial.
+    rewrite vis_restrict_sm, restrict_sm_all, restrict_nest; trivial. }
 
-  (* Ltailcall *)
+{ (* Ltailcall *)
   destruct ls0.
   rewrite vis_restrict_sm, restrict_sm_all, restrict_nest in AGREE; trivial.
   specialize (match_parent_locset0 _ _ rs0 _ STACKS); intros parentsAGREE.
@@ -2627,9 +2670,9 @@ Proof. intros.
            destruct H4; subst. 
            eapply visPropagate; try eassumption.
     eapply FreeEffect_PropagateLeft; try eassumption.
-    rewrite <- (stacksize_preserved _ _ TRF); eauto. 
+    rewrite <- (stacksize_preserved _ _ TRF); eauto. }
 
-  (* Lbuiltin*) 
+{ (* Lbuiltin*) 
   inv H. 
   assert (ArgsInj: val_list_inject (restrict (as_inj mu) (vis mu))
             (decode_longs (sig_args (ef_sig ef)) (reglist rs args))
@@ -2672,7 +2715,7 @@ Proof. intros.
       assert (FRG: frgnBlocksSrc mu = frgnBlocksSrc mu') by eapply INC.
           rewrite <- FRG. eapply (Glob _ H2).
   intros.
-    eapply BuiltinEffect_Propagate; try eassumption.
+    eapply BuiltinEffect_Propagate; try eassumption. }
 
   (* Lannot 
   eexists; eexists; split. 
@@ -2682,7 +2725,7 @@ Proof. intros.
   exact symbols_preserved. exact varinfo_preserved.
   econstructor; eauto.*)
 
-  (* Lbranch *)
+{ (* Lbranch *)
   eexists; eexists; eexists; split. 
   assert ((reachable f)!!pc = true). apply REACH; simpl; auto.
   right; split. simpl; omega. eapply effstep_star_zero.
@@ -2696,9 +2739,9 @@ Proof. intros.
       apply extensionality; intros; rewrite (freshloc_irrefl). intuition.
       apply extensionality; intros; rewrite (freshloc_irrefl). intuition.
   split; intuition.
-  split; intuition. econstructor; eauto. apply REACH. left. trivial. 
+  split; intuition. econstructor; eauto. apply REACH. left. trivial. }
 
-  (* Lcond *)
+{ (* Lcond *)
   rewrite vis_restrict_sm, restrict_sm_all, restrict_nest in AGREE; trivial.
   exploit eval_condition_inject; try eassumption.
     eapply agree_regs_list; try eassumption.
@@ -2779,8 +2822,9 @@ Proof. intros.
     split; intuition.
     split; intuition.
       econstructor; eauto.
-      rewrite vis_restrict_sm, restrict_sm_all, restrict_nest; trivial.
-  (* Ljumptable *)
+      rewrite vis_restrict_sm, restrict_sm_all, restrict_nest; trivial. }
+
+{ (* Ljumptable *)
   assert (REACH': (reachable f)!!pc = true).
     apply REACH. simpl. eapply list_nth_z_in; eauto. 
   eexists; eexists; eexists; split.
@@ -2795,9 +2839,9 @@ Proof. intros.
         apply extensionality; intros; rewrite (freshloc_irrefl). intuition.
         apply extensionality; intros; rewrite (freshloc_irrefl). intuition.
     split; intuition. 
-    split; intuition. econstructor; eauto.
+    split; intuition. econstructor; eauto. }
 
-  (* Lreturn *)
+{ (* Lreturn *)
   destruct ls0.
   rewrite vis_restrict_sm, restrict_sm_all, restrict_nest in AGREE; trivial.
   assert (WDR: SM_wd (restrict_sm mu (vis mu))).
@@ -2843,9 +2887,9 @@ Proof. intros.
            destruct H3; subst. 
            eapply visPropagate; try eassumption.
     eapply FreeEffect_PropagateLeft; try eassumption.
-    rewrite <- (stacksize_preserved _ _ TRF); eauto.  
+    rewrite <- (stacksize_preserved _ _ TRF); eauto. }
 
-  (* dummy step *)
+{ (* dummy step *)
   destruct ls0.
   assert (REACH: (reachable f)!!(LTL.fn_entrypoint f) = true).
     apply reachable_entrypoint.
@@ -2902,9 +2946,9 @@ Proof. intros.
           eapply intern_incr_as_inj; eassumption.
      assert (FF: frgnBlocksSrc mu = frgnBlocksSrc mu') by eapply IntInc.
        apply Glob in H1. rewrite <-FF; trivial.
-  intuition.
+  intuition. }
 
-  (* internal functions *)
+{ (* internal functions *)
   assert (REACH: (reachable f)!!(LTL.fn_entrypoint f) = true).
     apply reachable_entrypoint.
   monadInv H8.
@@ -2959,11 +3003,69 @@ Proof. intros.
           eapply intern_incr_as_inj; eassumption.
      assert (FF: frgnBlocksSrc mu = frgnBlocksSrc mu') by eapply IntInc.
        apply Glob in H1. rewrite <-FF; trivial.
-  intuition.
+  intuition. }
 
-  (* no external function *)
+{ contradiction. }
+{  (* unobservable external function *)
+  monadInv H9. inv H0.
+  rewrite vis_restrict_sm, restrict_sm_all in AGREE.
+  rewrite restrict_nest in AGREE; trivial.
+  assert (ArgsInj: val_list_inject (restrict (as_inj mu) (vis mu))
+            (decode_longs (sig_args (ef_sig ef)) (rs ## (Conventions1.loc_arguments (ef_sig ef))))
+            (decode_longs (sig_args (ef_sig ef)) (ls2 ## (Conventions1.loc_arguments (ef_sig ef))))).
+    simpl. eapply decode_longs_inject. 
+     eapply agree_regs_map_outgoing. assumption.
+     red; intros. apply Conventions1.loc_arguments_rec_charact in H0. 
+           destruct l; try contradiction.
+           destruct sl; try contradiction. trivial.
+  exploit (inlineable_extern_inject ge tge); try eassumption.
+  intros [mu' [v' [m'' [TEC [ResInj [MINJ' [UNMAPPED 
+         [LOOR [INC [SEP [LOCALLOC [WD' [SMV' RC']]]]]]]]]]]]].  
+  eexists; eexists m''; eexists.
+  split. left. apply effstep_plus_one. 
+          eapply lin_effexec_function_external; eauto.
+          econstructor; eauto.
+  exists mu'. 
+  split. assumption.
+  split. assumption.
+  split. assumption.
+  split.
+    { (*MATCH*)
+      split. 
+        econstructor; eauto.
+          eapply list_match_stackframes_intern_incr; try eassumption.
+           apply restrict_sm_intern_incr; eassumption.
+         eapply restrict_sm_WD; trivial.
+         rewrite vis_restrict_sm, restrict_sm_all; trivial.
+          rewrite restrict_nest; trivial.
+          eapply agree_regs_set_regs; try eassumption.
+          eapply agree_regs_incr; try eassumption.
+           eapply intern_incr_restrict; eassumption.
+          eapply encode_long_inject; eassumption.
+       intuition.
+       apply intern_incr_as_inj in INC; trivial.
+         apply sm_inject_separated_mem in SEP; trivial.
+         eapply meminj_preserves_incr_sep; eassumption. 
+       red; intros ? ? Hb. destruct (GFP _ _ Hb).
+          split; trivial.
+          eapply intern_incr_as_inj; eassumption.
+       assert (FRG: frgnBlocksSrc mu = frgnBlocksSrc mu') by eapply INC.
+          rewrite <- FRG. eapply (Glob _ H1). }
+  intros. 
+    exploit @BuiltinEffect_Propagate; try eapply H.
+      eassumption. 
+      eassumption. 
+      eassumption. 
+      instantiate (1:=ofs). instantiate (1:=b). instantiate (1:=tge).
+       unfold BuiltinEffect in H0; simpl in H0.
+       destruct ef; trivial. 
+    intros [VS EFF]. split; trivial. 
+    intros. destruct (EFF H1) as [b1 [d [FRG [EffB Perm]]]]; clear EFF. 
+     exists b1, d; repeat split; trivial. 
+       unfold BuiltinEffect in EffB; simpl in EffB. 
+       unfold BuiltinEffect; simpl. destruct ef; trivial. }
 
-  (* return *) 
+{ (* return *) 
   inv H5. inv H1.
   eexists; eexists; eexists; split.
   left. apply effstep_plus_one. econstructor.
@@ -2975,7 +3077,7 @@ Proof. intros.
       repeat split; extensionality b; 
           try rewrite (freshloc_irrefl); intuition.
       split. econstructor; eauto.
-    intuition.
+    intuition. }
 Qed.
 
 (*program structure not yet updated to module*)
@@ -2992,8 +3094,8 @@ Theorem transl_program_correct:
                 /\ Genv.find_funct_ptr ge b = Some f1
                 /\ Genv.find_funct_ptr tge b = Some f2)
          (init_mem: exists m0, Genv.init_mem prog = Some m0),
-SM_simulation.SM_simulation_inject LTL_eff_sem 
-  Linear_eff_sem ge tge entrypoints.
+SM_simulation.SM_simulation_inject (LTL_eff_sem  hf)
+  (Linear_eff_sem hf) ge tge entrypoints.
 Proof.
 intros.
 assert (GDE:= GDE_lemma). 
